TickTock/TickTock_Prefix.thy
@@ -182,9 +182,9 @@ proof auto
   qed
 qed
 
-lemma TT4_Prefix:
-  "TT4 P \<Longrightarrow> TT4 (e \<rightarrow>\<^sub>C P)"
-  unfolding PrefixTT_def TT4_def
+lemma TT3_Prefix:
+  "TT3 P \<Longrightarrow> TT3 (e \<rightarrow>\<^sub>C P)"
+  unfolding PrefixTT_def TT3_def
 proof auto
   fix s
   assume "s \<in> tocks {x. x \<noteq> Tock \<and> x \<noteq> Event e}"
@@ -192,14 +192,14 @@ proof auto
       (\<forall>\<sigma>\<in>P. add_Tick_refusal_trace s \<noteq> sa @ [Event e]\<^sub>E # \<sigma>) \<Longrightarrow>
     \<exists>sa\<in>tocks {x. x \<noteq> Tock \<and> x \<noteq> Event e}. \<exists>X. Tock \<notin> X \<and> Event e \<notin> X \<and> add_Tick_refusal_trace s = sa @ [[X]\<^sub>R]"
     apply (erule_tac x="add_Tick_refusal_trace s" in ballE, auto)
-    by (metis (mono_tags, lifting) TT4_def TT4_tocks ttevent.distinct(3) ttevent.simps(7) mem_Collect_eq)
+    by (metis (mono_tags, lifting) TT3_def TT3_tocks ttevent.distinct(3) ttevent.simps(7) mem_Collect_eq)
 next
   fix s X
   assume "s \<in> tocks {x. x \<noteq> Tock \<and> x \<noteq> Event e}" "Tock \<notin> X" "Event e \<notin> X"
   then show "\<exists>sa\<in>tocks {x. x \<noteq> Tock \<and> x \<noteq> Event e}.
     \<exists>Xa. Tock \<notin> Xa \<and> Event e \<notin> Xa \<and> add_Tick_refusal_trace (s @ [[X]\<^sub>R]) = sa @ [[Xa]\<^sub>R]"
     apply (rule_tac x="add_Tick_refusal_trace s" in bexI, rule_tac x="X \<union> {Tick}" in exI, auto simp add: add_Tick_refusal_trace_end_refusal)
-    by (metis (mono_tags, lifting) TT4_def TT4_tocks ttevent.distinct(3) ttevent.simps(7) mem_Collect_eq)
+    by (metis (mono_tags, lifting) TT3_def TT3_tocks ttevent.distinct(3) ttevent.simps(7) mem_Collect_eq)
 next
   fix s
   assume "s \<in> tocks {x. x \<noteq> Tock \<and> x \<noteq> Event e}"
@@ -207,7 +207,7 @@ next
       (\<forall>\<sigma>\<in>P. add_Tick_refusal_trace s \<noteq> sa @ [Event e]\<^sub>E # \<sigma>) \<Longrightarrow>
     \<exists>sa\<in>tocks {x. x \<noteq> Tock \<and> x \<noteq> Event e}. \<exists>X. Tock \<notin> X \<and> Event e \<notin> X \<and> add_Tick_refusal_trace s = sa @ [[X]\<^sub>R]"
     apply (erule_tac x="add_Tick_refusal_trace s" in ballE, auto)
-    by (metis (mono_tags, lifting) TT4_def TT4_tocks ttevent.distinct(3) ttevent.simps(7) mem_Collect_eq)
+    by (metis (mono_tags, lifting) TT3_def TT3_tocks ttevent.distinct(3) ttevent.simps(7) mem_Collect_eq)
 next
   fix s \<sigma>
   assume "s \<in> tocks {x. x \<noteq> Tock \<and> x \<noteq> Event e}" "\<sigma> \<in> P"
@@ -220,7 +220,7 @@ next
       \<exists>X. Tock \<notin> X \<and> Event e \<notin> X \<and> add_Tick_refusal_trace (s @ [Event e]\<^sub>E # \<sigma>) = sa @ [[X]\<^sub>R]"
     using calculation apply (erule_tac x="add_Tick_refusal_trace s" in ballE, auto)
     apply (erule_tac x="add_Tick_refusal_trace \<sigma>" in ballE, auto simp add: add_Tick_refusal_trace_end_event_trace)
-    by (metis (mono_tags, lifting) TT4_def TT4_tocks ttevent.distinct(3) ttevent.simps(7) mem_Collect_eq)
+    by (metis (mono_tags, lifting) TT3_def TT3_tocks ttevent.distinct(3) ttevent.simps(7) mem_Collect_eq)
 qed
 
 lemma TT_Prefix:
@@ -629,10 +629,10 @@ next
     done
 qed
 
-lemma TT4_TockPrefix:
-  assumes "TT4 P"
-  shows "TT4 (tock \<rightarrow>\<^sub>C P)"
-  unfolding TockPrefixTT_def TT4_def
+lemma TT3_TockPrefix:
+  assumes "TT3 P"
+  shows "TT3 (tock \<rightarrow>\<^sub>C P)"
+  unfolding TockPrefixTT_def TT3_def
 proof auto
   fix s :: "'a ttobs list"
   assume "s \<in> tocks {x. x \<noteq> Tock}"   
@@ -667,7 +667,7 @@ next
   then have 1: "add_Tick_refusal_trace s \<in> tocks {x. x \<noteq> Tock}"
     by (induct s rule:tocks.induct, auto simp add: tocks.intros)
   have 2: "add_Tick_refusal_trace \<sigma> \<in> P"
-    using assms case_assms unfolding TT4_def by auto
+    using assms case_assms unfolding TT3_def by auto
   show "\<forall>sa\<in>tocks {x. x \<noteq> Tock}. add_Tick_refusal_trace (s @ [X]\<^sub>R # [Tock]\<^sub>E # \<sigma>) \<noteq> sa \<and>
       (\<forall>\<sigma>'\<in>P. \<forall>Xa. Tock \<in> Xa \<or> add_Tick_refusal_trace (s @ [X]\<^sub>R # [Tock]\<^sub>E # \<sigma>) \<noteq> sa @ [Xa]\<^sub>R # [Tock]\<^sub>E # \<sigma>') \<Longrightarrow>
     \<exists>sa\<in>tocks {x. x \<noteq> Tock}. \<exists>Xa. Tock \<notin> Xa \<and> add_Tick_refusal_trace (s @ [X]\<^sub>R # [Tock]\<^sub>E # \<sigma>) = sa @ [[Xa]\<^sub>R]"
@@ -677,7 +677,7 @@ next
 qed
 
 lemma TT_TockPrefix:
-  assumes "TT P" "TT2 P" "TT4 P"
+  assumes "TT P" "TT2 P" "TT3 P"
   shows "TT (tock \<rightarrow>\<^sub>C P)"
   using assms unfolding TT_def
   using TT0_TockPrefixTT TT1_TockPrefixTT TT2_TockPrefix TT2_imp_TT2w ttWFx_TockPrefix TockPrefixTT_wf by blast
